Replace use of state by memory, and change memory type

src/arch/x64/X64.Memory_i_s.fst
@@ -1,6 +1,6 @@
 module X64.Memory_i_s
 
-
+module I = Interop64
 module HS = FStar.HyperStack
 module B = FStar.Buffer
 module M = FStar.Modifies
@@ -8,7 +8,14 @@ module S = X64.Bytes_Semantics_s
 module H = FStar.Heap
 
 let heap = H.heap
-let mem = HS.mem
+noeq type mem' = {
+  addrs : I.addr_map;
+  ptrs : list (B.buffer UInt64.t);
+  hs : HS.mem;
+  }
+
+type mem = (m:mem'{I.list_disjoint_or_eq #UInt64.t m.ptrs /\
+  I.list_live m.hs m.ptrs})
 
 let op_String_Access = Map.sel
 let op_String_Assignment = Map.upd
@@ -61,12 +68,13 @@ let lemma_v_to_of_typ (t:typ) (v:type_of_typ t) : Lemma
 let buffer t = B.buffer (m_of_typ t)
 
 let buffer_as_seq #t h b =
-  let s = B.as_seq h b in
+  let s = B.as_seq h.hs b in
   let len = Seq.length s in
   let contents (i:nat{i < len}) : type_of_typ t = v_to_typ t (Seq.index s i) in
   Seq.init len contents
 
-let buffer_readable #t h b = B.live h b
+// TODO: Fix this
+let buffer_readable #t h b = if (t = TBase TUInt64) then List.memP b h.ptrs else false
 let buffer_length #t b = B.length b
 let loc = M.loc
 let loc_none = M.loc_none
@@ -74,14 +82,11 @@ let loc_union = M.loc_union
 let loc_buffer #t b = M.loc_buffer b
 let loc_disjoint = M.loc_disjoint
 let loc_includes = M.loc_includes
-let modifies = M.modifies
-
-let valid_state s = 
-  // Shouldn't be needed but logic annotation issue without it
+let modifies s h h' = 
   let _ = () in
-  I.list_disjoint_or_eq #UInt64.t s.ptrs /\
-  I.list_live s.mem s.ptrs /\
-  s.state.S.mem == I.down_mem64 s.mem s.addrs s.ptrs
+  M.modifies s h.hs h'.hs /\ h.ptrs == h'.ptrs /\ h.addrs == h'.addrs
+
+let valid_state s = s.state.S.mem == I.down_mem64 s.mem.hs s.mem.addrs s.mem.ptrs
 
 let loc_readable h s = unit // admit()
 let loc_readable_none = admit()
@@ -110,7 +115,7 @@ let modifies_loc_readable #t b p h h' =
 let modifies_buffer_elim #t1 b p h h' =
   if buffer_length b > 0 then
   (
-    M.modifies_buffer_elim b p h h';
+    M.modifies_buffer_elim b p h.hs h'.hs;
     assert (Seq.equal (buffer_as_seq h b) (buffer_as_seq h' b));
     ()
   )
@@ -129,10 +134,10 @@ let loc_includes_union_r s s1 s2 = M.loc_includes_union_r s s1 s2
 let loc_includes_union_l s1 s2 s = M.loc_includes_union_l s1 s2 s
 let loc_includes_union_l_buffer #t s1 s2 b = M.loc_includes_union_l s1 s2 (loc_buffer b)
 let loc_includes_none s = M.loc_includes_none s
-let modifies_refl s h = M.modifies_refl s h
-let modifies_goal_directed_refl s h = M.modifies_refl s h
-let modifies_loc_includes s1 h h' s2 = M.modifies_loc_includes s1 h h' s2
-let modifies_trans s12 h1 h2 s23 h3 = M.modifies_trans s12 h1 h2 s23 h3
+let modifies_refl s h = M.modifies_refl s h.hs
+let modifies_goal_directed_refl s h = M.modifies_refl s h.hs
+let modifies_loc_includes s1 h h' s2 = M.modifies_loc_includes s1 h.hs h'.hs s2
+let modifies_trans s12 h1 h2 s23 h3 = M.modifies_trans s12 h1.hs h2.hs s23 h3.hs
 
 let modifies_goal_directed_trans s12 h1 h2 s13 h3 =
   modifies_trans s12 h1 h2 s13 h3;
@@ -164,26 +169,27 @@ let buffer_write #t b i v h =
  if i < 0 || i >= buffer_length b then h else
  begin
  let vu = v_of_typ t v in
- let s0 = B.sel h b in
+ let s0 = B.sel h.hs b in
  let s = Seq.upd s0 (B.idx b + i) vu in
- let h' = HS.upd h (B.content b) s in
- lemma_aux b i vu h;
+ let h' = HS.upd h.hs (B.content b) s in
+ let h' = {h with hs = h'} in
+ lemma_aux b i vu h.hs;
  assert (Seq.equal (buffer_as_seq h' b) (Seq.upd (buffer_as_seq h b) i v));
  h'
  end
 
-let buffer_addr #t b s =
-  let addrs = s.addrs in
+let buffer_addr #t b h =
+  let addrs = h.addrs in
   addrs.[(B.as_addr b, B.idx b, B.length b)]
 
-val addr_in_ptr: (addr:int) -> (ptr:buffer64) -> (s:state) ->
+val addr_in_ptr: (addr:int) -> (ptr:buffer64) -> (h:mem) ->
   GTot (b:bool{ not b <==> (forall i. 0 <= i /\ i < B.length ptr ==> 
-    addr <> (buffer_addr ptr s) + 8 `op_Multiply` i)})
+    addr <> (buffer_addr ptr h) + 8 `op_Multiply` i)})
   
 // Checks if address addr corresponds to one of the elements of buffer ptr
-let addr_in_ptr (addr:int) (ptr:buffer64) (s:state) =
+let addr_in_ptr (addr:int) (ptr:buffer64) (h:mem) =
   let n = B.length ptr in
-  let base = buffer_addr ptr s in
+  let base = buffer_addr ptr h in
   let rec aux (i:nat) : Tot (b:bool{not b <==> (forall j. i <= j /\ j < n ==> 
     addr <> base + 8 `op_Multiply` j)}) 
     (decreases %[n-i]) =
@@ -200,60 +206,60 @@ let rec get_addr_in_ptr (n base addr:nat) (i:nat{exists j. i <= j /\ j < n /\ ba
     else get_addr_in_ptr n base addr (i+1)
 
 
-let rec valid_mem_aux addr ps (s:state) : GTot (b:bool{
-  (not b) <==> (forall (x:buffer64). (List.memP x ps ==> not (addr_in_ptr addr x s) ))}) 
+let rec valid_mem_aux addr ps (h:mem) : GTot (b:bool{
+  (not b) <==> (forall (x:buffer64). (List.memP x ps ==> not (addr_in_ptr addr x h) ))}) 
   = match ps with
     | [] -> false
-    | a::q -> if (addr_in_ptr addr a s) then true else valid_mem_aux addr q s
+    | a::q -> if (addr_in_ptr addr a h) then true else valid_mem_aux addr q h
 
-let valid_mem64 ptr s = valid_mem_aux ptr s.ptrs s
+let valid_mem64 ptr h = valid_mem_aux ptr h.ptrs h
 
 // TODO: Probably a similar approach baser on buffer_read?
-let load_mem64 ptr s = S.get_heap_val64 ptr s.state.S.mem
+let load_mem64 ptr s = admit() //S.get_heap_val64 ptr s.state.S.mem
 
-let rec store_mem_aux addr ps (v:nat64) (s:state) (h0:HS.mem{I.list_live h0 ps}) : 
-  GTot (h1:HS.mem{forall (b:buffer64). B.live h0 b <==> B.live h1 b }) =
+let rec store_mem_aux addr (ps:list buffer64) (v:nat64) (h:mem{forall x. List.memP x ps ==> List.memP x h.ptrs }) : 
+  GTot (h1:mem{forall (b:buffer64). B.live h.hs b <==> B.live h1.hs b }) =
   match ps with
-  | [] -> h0
+  | [] -> h
   | a::q ->
-    let base = buffer_addr a s in
+    let base = buffer_addr a h in
     let n = B.length a in
-    if addr_in_ptr addr a s then
+    if addr_in_ptr addr a h then
     begin
-      buffer_write a (get_addr_in_ptr n base addr 0) v h0
+      buffer_write a (get_addr_in_ptr n base addr 0) v h
     end
-    else store_mem_aux addr q v s h0
+    else store_mem_aux addr q v h
 
 #set-options "--z3rlimit 40"
 
 let rec written_buffer_down_aux1 (b:buffer64) (i:nat{i < B.length b}) (v:nat64)
       (ps:list buffer64{I.list_disjoint_or_eq ps /\ List.memP b ps})
-      (h0:HS.mem{I.list_live h0 ps}) (s:state)
-      (base:nat{base == buffer_addr b s})
-      (k:nat) (h1:HS.mem{h1 == buffer_write b i v h0}) 
-      (mem1:S.heap{I.correct_down64 h0 s.addrs ps mem1}) 
+      (h:mem{forall x. List.memP x ps ==> List.memP x h.ptrs})
+      (base:nat{base == buffer_addr b h})
+      (k:nat) (h1:mem{h1 == buffer_write b i v h}) 
+      (mem1:S.heap{I.correct_down64 h.hs h.addrs ps mem1}) 
       (mem2:S.heap{
-      (I.correct_down64 h1 s.addrs ps mem2) /\
+      (I.correct_down64 h1.hs h.addrs ps mem2) /\
       (forall j. base <= j /\ j < base + k `op_Multiply` 8 ==> mem1.[j] == mem2.[j])}) : 
       Lemma (requires True)
       (ensures (forall j. j >= base /\ j < base + 8 `op_Multiply` i ==> mem1.[j] == mem2.[j]))
       (decreases %[i-k]) =
     if k >= i then ()
     else begin
-      assert (Seq.index (B.as_seq h0 b) k == Seq.index (B.as_seq h1 b) k);
+      assert (Seq.index (B.as_seq h.hs b) k == Seq.index (B.as_seq h1.hs b) k);
       Bytes_Semantics_i.same_mem_get_heap_val (base + 8 `op_Multiply` k) mem1 mem2;
-      written_buffer_down_aux1 b i v ps h0 s base (k+1) h1 mem1 mem2
+      written_buffer_down_aux1 b i v ps h base (k+1) h1 mem1 mem2
     end
 
 let rec written_buffer_down_aux2 (b:buffer64) (i:nat{i < B.length b}) (v:nat64)
       (ps:list buffer64{I.list_disjoint_or_eq ps /\ List.memP b ps})
-      (h0:HS.mem{I.list_live h0 ps}) (s:state)
-      (base:nat{base == buffer_addr b s})
+      (h:mem{forall x. List.memP x ps ==> List.memP x h.ptrs})
+      (base:nat{base == buffer_addr b h})
       (n:nat{n == B.length b})
-      (k:nat{k > i}) (h1:HS.mem{h1 == buffer_write b i v h0}) 
-      (mem1:S.heap{I.correct_down64 h0 s.addrs ps mem1}) 
+      (k:nat{k > i}) (h1:mem{h1 == buffer_write b i v h}) 
+      (mem1:S.heap{I.correct_down64 h.hs h.addrs ps mem1}) 
       (mem2:S.heap{
-      (I.correct_down64 h1 s.addrs ps mem2) /\
+      (I.correct_down64 h1.hs h.addrs ps mem2) /\
       (forall j. base + 8 `op_Multiply` (i+1) <= j /\ j < base + k `op_Multiply` 8 ==>
       mem1.[j] == mem2.[j])}) :
       Lemma 
@@ -263,29 +269,29 @@ let rec written_buffer_down_aux2 (b:buffer64) (i:nat{i < B.length b}) (v:nat64)
       (decreases %[n-k]) =
     if k >= n then ()
     else begin
-      assert (Seq.index (B.as_seq h0 b) k == Seq.index (B.as_seq h1 b) k);
+      assert (Seq.index (B.as_seq h.hs b) k == Seq.index (B.as_seq h1.hs b) k);
       Bytes_Semantics_i.same_mem_get_heap_val (base + 8 `op_Multiply` k) mem1 mem2;
-      written_buffer_down_aux2 b i v ps h0 s base n (k+1) h1 mem1 mem2
+      written_buffer_down_aux2 b i v ps h base n (k+1) h1 mem1 mem2
     end
     
 let written_buffer_down (b:buffer64) (i:nat{i < B.length b}) (v:nat64)
-  (ps: list buffer64{I.list_disjoint_or_eq ps /\ List.memP b ps}) (h0:HS.mem{I.list_live h0 ps}) (s:state) :
+  (ps: list buffer64{I.list_disjoint_or_eq ps /\ List.memP b ps}) (h:mem{forall x. List.memP x ps ==> List.memP x h.ptrs}) :
   Lemma (
-    let mem1 = I.down_mem64 h0 s.addrs ps in
-    let h1 = buffer_write b i v h0 in
-    let mem2 = I.down_mem64 h1 s.addrs ps in
-    let base = buffer_addr b s in
+    let mem1 = I.down_mem64 h.hs h.addrs ps in
+    let h1 = buffer_write b i v h in
+    let mem2 = I.down_mem64 h1.hs h.addrs ps in
+    let base = buffer_addr b h in
     let n = B.length b in
     forall j. (base <= j /\ j < base + 8 `op_Multiply` i) \/ 
 	 (base + 8 `op_Multiply` (i+1) <= j /\ j < base + 8 `op_Multiply` n) ==>
 	 mem1.[j] == mem2.[j]) = 
-    let mem1 = I.down_mem64 h0 s.addrs ps in
-    let h1 = buffer_write b i v h0 in
-    let mem2 = I.down_mem64 h1 s.addrs ps in	 
-    let base = buffer_addr b s in
+    let mem1 = I.down_mem64 h.hs h.addrs ps in
+    let h1 = buffer_write b i v h in
+    let mem2 = I.down_mem64 h1.hs h.addrs ps in	 
+    let base = buffer_addr b h in
     let n = B.length b in
-    written_buffer_down_aux1 b i v ps h0 s base 0 h1 mem1 mem2;
-    written_buffer_down_aux2 b i v ps h0 s base n (i+1) h1 mem1 mem2
+    written_buffer_down_aux1 b i v ps h base 0 h1 mem1 mem2;
+    written_buffer_down_aux2 b i v ps h base n (i+1) h1 mem1 mem2
 
 let same_mem_get_heap_val_buf (base n:int) (mem1 mem2:S.heap) : Lemma
   (requires (forall i. 0 <= i /\ i < n ==> 
@@ -307,126 +313,123 @@ let same_mem_get_heap_val_buf (base n:int) (mem1 mem2:S.heap) : Lemma
 
 let rec unwritten_buffer_down_aux (b:buffer64) (i:nat{i < B.length b}) (v:nat64)
   (ps: list buffer64{I.list_disjoint_or_eq ps /\ List.memP b ps})
-  (h0:HS.mem{I.list_live h0 ps}) 
-  (s:state) (a:buffer64{a =!= b /\ List.memP a ps})  : 
-  Lemma (let base = buffer_addr a s in
-    let mem1 = I.down_mem64 h0 s.addrs ps in
-    let h1 = buffer_write b i v h0 in
-    let mem2 = I.down_mem64 h1 s.addrs ps in
+  (h:mem{forall x. List.memP x ps ==> List.memP x h.ptrs})
+  (a:buffer64{a =!= b /\ List.memP a ps})  : 
+  Lemma (let base = buffer_addr a h in
+    let mem1 = I.down_mem64 h.hs h.addrs ps in
+    let h1 = buffer_write b i v h in
+    let mem2 = I.down_mem64 h1.hs h.addrs ps in
     forall j. j >= base /\ j < base + (B.length a) `op_Multiply` 8 ==> mem1.[j] == mem2.[j]) =
-    let mem1 = I.down_mem64 h0 s.addrs ps in
-    let h1 = buffer_write b i v h0 in
-    let mem2 = I.down_mem64 h1 s.addrs ps in
-    let base = buffer_addr a s in    
-    let s0 = B.as_seq h0 a in
+    let mem1 = I.down_mem64 h.hs h.addrs ps in
+    let h1 = buffer_write b i v h in
+    let mem2 = I.down_mem64 h1.hs h.addrs ps in
+    let base = buffer_addr a h in    
+    let s0 = B.as_seq h.hs a in
     assert (I.disjoint_or_eq a b);
     // We need this to help z3
     assert (forall j. 0 <= j /\ j < B.length a ==> UInt64.v (Seq.index s0 j) == S.get_heap_val64 (base + (j `op_Multiply` 8)) mem1 );
     same_mem_get_heap_val_buf base (B.length a) mem1 mem2
 
 let unwritten_buffer_down (b:buffer64) (i:nat{i < B.length b}) (v:nat64)
-  (ps: list buffer64{I.list_disjoint_or_eq ps /\ List.memP b ps}) (h0:HS.mem{I.list_live h0 ps}) (s:state) : Lemma (
-    let mem1 = I.down_mem64 h0 s.addrs ps in
-    let h1 = buffer_write b i v h0 in
-    let mem2 = I.down_mem64 h1 s.addrs ps in
+  (ps: list buffer64{I.list_disjoint_or_eq ps /\ List.memP b ps}) 
+  (h:mem{forall x. List.memP x ps ==> List.memP x h.ptrs}) : Lemma (
+    let mem1 = I.down_mem64 h.hs h.addrs ps in
+    let h1 = buffer_write b i v h in
+    let mem2 = I.down_mem64 h1.hs h.addrs ps in
     forall  (a:buffer64{List.memP a ps /\ a =!= b}) j.
-    let base = buffer_addr a s in j >= base /\ j < base + B.length a `op_Multiply` 8 ==> mem1.[j] == mem2.[j]) =
-    let mem1 = I.down_mem64 h0 s.addrs ps in
-    let h1 = buffer_write b i v h0 in
-    let mem2 = I.down_mem64 h1 s.addrs ps in   
+    let base = buffer_addr a h in j >= base /\ j < base + B.length a `op_Multiply` 8 ==> mem1.[j] == mem2.[j]) =
+    let mem1 = I.down_mem64 h.hs h.addrs ps in
+    let h1 = buffer_write b i v h in
+    let mem2 = I.down_mem64 h1.hs h.addrs ps in   
     let fintro (a:buffer64{List.memP a ps /\ a =!= b}) 
       : Lemma 
-      (forall j. let base = buffer_addr a s in 
+      (forall j. let base = buffer_addr a h in 
       j >= base /\ j < base + (B.length a) `op_Multiply` 8 ==> 
 	mem1.[j] == mem2.[j]) =
-      let base = buffer_addr a s in
-      unwritten_buffer_down_aux b i v ps h0 s a
+      let base = buffer_addr a h in
+      unwritten_buffer_down_aux b i v ps h a
     in
     Classical.forall_intro fintro
 
 let store_buffer_down_mem (b:buffer64) (i:nat{i < B.length b}) (v:nat64)
-  (ps: list buffer64{I.list_disjoint_or_eq ps /\ List.memP b ps}) (h0:HS.mem{I.list_live h0 ps}) (s:state) :
+  (ps: list buffer64{I.list_disjoint_or_eq ps /\ List.memP b ps})
+  (h:mem{forall x. List.memP x ps ==> List.memP x h.ptrs}) :
   Lemma (
-    let mem1 = I.down_mem64 h0 s.addrs ps in
-    let h1 = buffer_write b i v h0 in
-    let mem2 = I.down_mem64 h1 s.addrs ps in
-    let base = buffer_addr b s in
+    let mem1 = I.down_mem64 h.hs h.addrs ps in
+    let h1 = buffer_write b i v h in
+    let mem2 = I.down_mem64 h1.hs h.addrs ps in
+    let base = buffer_addr b h in
     forall j. j < base + 8 `op_Multiply` i \/ j >= base + 8 `op_Multiply` (i+1) ==>
       mem1.[j] == mem2.[j]) =
-    let mem1 = I.down_mem64 h0 s.addrs ps in
-    let h1 = buffer_write b i v h0 in
-    let mem2 = I.down_mem64 h1 s.addrs ps in
-    let base = buffer_addr b s in
+    let mem1 = I.down_mem64 h.hs h.addrs ps in
+    let h1 = buffer_write b i v h in
+    let mem2 = I.down_mem64 h1.hs h.addrs ps in
+    let base = buffer_addr b h in
     let n = B.length b in
-    I.same_unspecified_down h0 h1 s.addrs ps;
-    unwritten_buffer_down b i v ps h0 s;
-    assert (forall j. (exists (a:buffer64{List.memP a ps /\ a =!= b}) . let base = buffer_addr a s in
+    I.same_unspecified_down h.hs h1.hs h.addrs ps;
+    unwritten_buffer_down b i v ps h;
+    assert (forall j. (exists (a:buffer64{List.memP a ps /\ a =!= b}) . let base = buffer_addr a h in
       j >= base /\ j < base + B.length a `op_Multiply` 8) ==> mem1.[j] == mem2.[j]);
 
-    written_buffer_down b i v ps h0 s;
+    written_buffer_down b i v ps h;
     ()
 
-let rec get_addr_ptr (ptr:int) (s:state) (ps:list buffer64{valid_mem_aux ptr ps s}) : 
-  GTot (b:buffer64{List.memP b ps /\ addr_in_ptr ptr b s}) =
+let rec get_addr_ptr (ptr:int) (h:mem) (ps:list buffer64{valid_mem_aux ptr ps h}) : 
+  GTot (b:buffer64{List.memP b ps /\ addr_in_ptr ptr b h}) =
   match ps with
   // The list cannot be empty because of the mem predicate
-  | a::q -> if addr_in_ptr ptr a s then a else get_addr_ptr ptr s q
+  | a::q -> if addr_in_ptr ptr a h then a else get_addr_ptr ptr h q
 
-let store_buffer_aux_down_mem (ptr:int) (v:nat64) (s:state{valid_mem64 ptr s}) : Lemma (
-  let mem1 = I.down_mem64 s.mem s.addrs s.ptrs in
-  let h1 = store_mem_aux ptr s.ptrs v s s.mem in
-  let mem2 = I.down_mem64 h1 s.addrs s.ptrs in
+let store_buffer_aux_down_mem (ptr:int) (v:nat64) (h:mem{valid_mem64 ptr h}) : Lemma (
+  let mem1 = I.down_mem64 h.hs h.addrs h.ptrs in
+  let h1 = store_mem_aux ptr h.ptrs v h in
+  let mem2 = I.down_mem64 h1.hs h.addrs h.ptrs in
   forall j. j < ptr \/ j >= ptr + 8 ==> mem1.[j] == mem2.[j]) =
-  let h1 = store_mem_aux ptr s.ptrs v s s.mem in
-  let b = get_addr_ptr ptr s s.ptrs in
-  let i = get_addr_in_ptr (B.length b) (buffer_addr b s) ptr 0 in
-  let rec aux (ps:list buffer64{I.list_disjoint_or_eq ps /\ valid_mem_aux ptr ps s}) (h:HS.mem{I.list_live h ps}) :
-  Lemma (let b = get_addr_ptr ptr s ps in
-    let i = get_addr_in_ptr (B.length b) (buffer_addr b s) ptr 0 in
-    store_mem_aux ptr ps v s h == buffer_write b i v h) =
+  let h1 = store_mem_aux ptr h.ptrs v h in
+  let b = get_addr_ptr ptr h h.ptrs in
+  let i = get_addr_in_ptr (B.length b) (buffer_addr b h) ptr 0 in
+  let rec aux (ps:list buffer64{I.list_disjoint_or_eq ps /\ valid_mem_aux ptr ps h}) 
+  (h0:mem{h0.addrs == h.addrs /\ (forall x. List.memP x ps ==> List.memP x h0.ptrs)}) :
+  Lemma (let b = get_addr_ptr ptr h ps in
+    let i = get_addr_in_ptr (B.length b) (buffer_addr b h) ptr 0 in
+    store_mem_aux ptr ps v h0 == buffer_write b i v h0) =
     match ps with
     | [] -> ()
     | a::q ->
-      if addr_in_ptr ptr a s then () else aux q h    
-  in aux s.ptrs s.mem;
-  store_buffer_down_mem b i v s.ptrs s.mem s
+      if addr_in_ptr ptr a h0 then () else aux q h0    
+  in aux h.ptrs h;
+  store_buffer_down_mem b i v h.ptrs h
 
-let store_buffer_aux_down_mem2 (ptr:int) (v:nat64) (s:state{valid_mem64 ptr s}) : Lemma (
-  let h1 = store_mem_aux ptr s.ptrs v s s.mem in
-  let mem2 = I.down_mem64 h1 s.addrs s.ptrs in
+let store_buffer_aux_down_mem2 (ptr:int) (v:nat64) (h:mem{valid_mem64 ptr h}) : Lemma (
+  let h1 = store_mem_aux ptr h.ptrs v h in
+  let mem2 = I.down_mem64 h1.hs h.addrs h.ptrs in
   S.get_heap_val64 ptr mem2 == v) =
-  let b = get_addr_ptr ptr s s.ptrs in
-  let i = get_addr_in_ptr (B.length b) (buffer_addr b s) ptr 0 in
-  let h1 = store_mem_aux ptr s.ptrs v s s.mem in
-  let mem2 = I.down_mem64 h1 s.addrs s.ptrs in
-  let rec aux (ps:list buffer64{I.list_disjoint_or_eq ps /\ valid_mem_aux ptr ps s}) (h:HS.mem{I.list_live h ps}) :
-  Lemma (let b = get_addr_ptr ptr s ps in
-    let i = get_addr_in_ptr (B.length b) (buffer_addr b s) ptr 0 in
-    store_mem_aux ptr ps v s h == buffer_write b i v h) =
+  let b = get_addr_ptr ptr h h.ptrs in
+  let i = get_addr_in_ptr (B.length b) (buffer_addr b h) ptr 0 in
+  let h1 = store_mem_aux ptr h.ptrs v h in
+  let mem2 = I.down_mem64 h1.hs h.addrs h.ptrs in
+  let rec aux (ps:list buffer64{I.list_disjoint_or_eq ps /\ valid_mem_aux ptr ps h}) 
+  (h0:mem{h0.addrs == h.addrs /\ (forall x. List.memP x ps ==> List.memP x h0.ptrs)}) :
+  Lemma (let b = get_addr_ptr ptr h ps in
+    let i = get_addr_in_ptr (B.length b) (buffer_addr b h) ptr 0 in
+    store_mem_aux ptr ps v h0 == buffer_write b i v h0) =
     match ps with
     | [] -> ()
     | a::q ->
-      if addr_in_ptr ptr a s then () else aux q h    
-  in aux s.ptrs s.mem;
-  assert (UInt64.v (Seq.index (B.as_seq h1 b) i) == v);
+      if addr_in_ptr ptr a h0 then () else aux q h0    
+  in aux h.ptrs h;
+  assert (UInt64.v (Seq.index (B.as_seq h1.hs b) i) == v);
   ()
 
 #set-options "--z3rlimit 60"
 
-let store_mem64 i v s =
-  if not (valid_mem64 i s) then s
+let store_mem64 i v h =
+  if not (valid_mem64 i h) then h
   else
-  let s' = S.update_mem i v s.state in
-  let h1 = store_mem_aux i s.ptrs v s s.mem in
-  let s' = {s with state = s'; mem = h1} in
-  Bytes_Semantics_i.frame_update_heap i v s.state.S.mem;
-  store_buffer_aux_down_mem i v s;
-  store_buffer_aux_down_mem2 i v s;
-  let mem1 = s'.state.S.mem in
-  let mem2 = I.down_mem64 s'.mem s.addrs s.ptrs in
-  Bytes_Semantics_i.same_mem_get_heap_val i mem1 mem2;
-  Bytes_Semantics_i.correct_update_get i v s.state.S.mem;
-  assert (forall j. mem1.[j] == mem2.[j]);
-  assert (Map.equal mem1 mem2);
-  s'
+  let h1 = store_mem_aux i h.ptrs v h in
+  h1
+
+let valid_mem128 ptr h = admit()
+let load_mem128 ptr h = admit()
+let store_mem128 ptr v h = admit()
 
